PrefixedEngine: move to the Meta.v file

Engine/Prefix.v
@@ -14,12 +14,6 @@ From Linden Require Import Parameters LWParameters.
 From Linden Require Import StrictSuffix.
 From Warblre Require Import Base RegExpRecord.
 
-From Linden Require Import PikeSubset SeenSets.
-From Linden Require Import Correctness FunctionalPikeVM.
-
-Section Prefix.
-  Context {params: LindenParameters}.
-
 (* Tactic for rewriting decidable equalities into propositional ones *)
 Ltac wt_eq := repeat match goal with
   | [ H: (?x ==? ?y)%wt = true |- _ ] => rewrite EqDec.inversion_true in H; subst
@@ -27,6 +21,9 @@ Ltac wt_eq := repeat match goal with
   | [ |- context[(?x ==? ?y)%wt] ] => destruct (x ==? y)%wt eqn:?Heq
   | [ H: context[(?x ==? ?y)%wt] |- _ ] => destruct (x ==? y)%wt eqn:?Heq
 end.
+
+Section Prefix.
+  Context {params: LindenParameters}.
 
 Inductive starts_with: string -> string -> Prop :=
 | sw_nil: forall s, starts_with [] s
@@ -198,7 +195,7 @@ Proof.
 Qed.
 
 (* low inclusive, high exclusive *)
-Notation input_between ilow ihigh i := ((i = ilow \/ strict_suffix i ilow forward) /\ strict_suffix ihigh i forward).
+Definition input_between ilow ihigh i := ((i = ilow \/ strict_suffix i ilow forward) /\ strict_suffix ihigh i forward).
 
 (* if strict_suffix i2 i1 forward, then next_str i2 is skipn k (next_str i1) for some k > 0 *)
 Lemma strict_suffix_forward_skipn:
@@ -826,214 +823,4 @@ Proof.
 Qed.
 
 End Literal.
-
-Section PrefixedEngine.
-  Context (rer: RegExpRecord).
-  Context {VMS: VMSeen}.
-  Context (no_i_flag : RegExpRecord.ignoreCase rer = false).
-
-(* interface of an executable engine *)
-Class Engine := {
-  exec: regex -> input -> option leaf;
-
-  (* asserts the supported subset of regexes *)
-  supported_regex: regex -> Prop;
-
-  (* the execution follows the backtracking tree semantics *)
-  exec_correct: forall r inp ol,
-    supported_regex r ->
-      ((exists tree,
-        is_tree rer [Areg r] inp Groups.GroupMap.empty forward tree /\
-        first_leaf tree inp = ol) <->
-      exec r inp = ol)
-}.
-
-(* relation that one input is a non-strict prefix of another *)
-Inductive input_prefix : input -> input -> Prop :=
-| ip_eq : forall inp, input_prefix inp inp
-| ip_prev : forall inp1 inp2 inp3,
-    advance_input inp1 forward = Some inp2 ->
-    input_prefix inp2 inp3 ->
-    input_prefix inp1 inp3.
-
-Lemma ip_prev':
-  forall inp1 inp2 inp3,
-    input_prefix inp1 inp2 ->
-    advance_input inp2 forward = Some inp3 ->
-    input_prefix inp1 inp3.
-Proof. induction 1; eauto using ip_prev, ip_eq. Qed.
-
-(* equivalence between input_prefix and strict_suffix *)
-Lemma input_prefix_strict_suffix:
-  forall i1 i2,
-    input_prefix i1 i2 <->
-      i2 = i1 \/ strict_suffix i2 i1 forward.
-Proof.
-  split; intros H.
-  - induction H; [auto|].
-    destruct IHinput_prefix; subst; eauto using ss_advance, ss_next'.
-  - destruct H; [subst; auto using ip_eq|].
-    remember forward as dir.
-    induction H; subst; eauto using ip_eq, ip_prev, ip_prev'.
-Qed.
-
-(* for each input position we run the engine and return the earliest match *)
-Fixpoint search_from {engine:Engine} (r: regex) (next: string) (prev: string): option leaf :=
-  match (exec r (Input next prev)) with
-  | Some leaf => Some leaf
-  | None => match next with
-            | [] => None
-            | c::t => search_from r t (c::prev)
-            end
-  end.
-
-Definition pref_str (i: input) : string :=
-  match i with
-  | Input _ pref => pref
-  end.
-
-(* the string-quadratic algorithm described in RegExpBuiltinExec *)
-Definition BuiltinExec {engine:Engine} (r:regex) (inp:input) : option leaf :=
-  search_from r (next_str inp) (pref_str inp).
-
-(* prefixed version *)
-Definition BuiltinExecPrefixed {strs:StrSearch} {engine:Engine} (r:regex) (inp:input) : option leaf :=
-  let lit := extract_literal r in
-  if lit == Impossible then None else
-    let p := prefix lit in
-    (* we skip the initial input that does not match the prefix *)
-    match (input_search p inp) with
-    | None => None (* if prefix is not present anywhere, then we cannot match *)
-    | Some i => search_from r (next_str i) (pref_str i)
-    end.
-
-Lemma search_from_before_jump_eq {strs:StrSearch} {engine:Engine}:
-  forall i r inp inp',
-    supported_regex r ->
-    input_search (prefix (extract_literal r)) inp = Some inp' ->
-    input_prefix i inp' ->
-    input_prefix inp i ->
-    search_from r (next_str i) (pref_str i) = search_from r (next_str inp') (pref_str inp').
-Proof.
-  intros i r inp inp' Hsubset Hsearch Hprefix Hlow.
-  induction Hprefix.
-  - reflexivity.
-  - pose proof H as Hadvance.
-    specialize (IHHprefix Hsearch).
-    unfold advance_input in H. destruct inp1 as [next1 pref1] eqn:Hinp1, next1 eqn:Hnext1; [easy|].
-    inversion H. rewrite <-H1 in IHHprefix.
-
-    assert (Hnone: exec r (Input (t :: s) pref1) = None). {
-      assert (Hbetween: input_between inp inp3 inp1). {
-        rewrite input_prefix_strict_suffix in Hprefix, Hlow.
-        split; destruct Hprefix, Hlow; subst; eauto using ss_next', ss_advance.
-      }
-
-      subst.
-      pose proof (is_tree_productivity r (Input (t :: s) pref1) Groups.GroupMap.empty forward) as [tree Htree].
-      rewrite <-exec_correct; [|assumption].
-      eauto using input_search_no_earlier, extract_literal_prefix_contra.
-    }
-    simpl.
-    rewrite Hnone.
-    eauto using ip_prev'.
-Qed.
-
-Lemma input_search_exec_none {strs:StrSearch} {engine:Engine}:
-  forall i r inp,
-    supported_regex r ->
-    input_search (prefix (extract_literal r)) inp = None ->
-    input_prefix inp i ->
-    exec r i = None.
-Proof.
-  intros i r inp Hsubset Hsearch Hlow.
-  rewrite input_prefix_strict_suffix in Hlow.
-  rewrite <-exec_correct; [|assumption].
-  pose proof (is_tree_productivity r i Groups.GroupMap.empty forward) as [tree Htree].
-  eauto using input_search_not_found, extract_literal_prefix_contra.
-Qed.
-
-Lemma search_from_none_prefix {strs:StrSearch} {engine:Engine}:
-  forall i r inp,
-    supported_regex r ->
-    input_search (prefix (extract_literal r)) inp = None ->
-    input_prefix inp i ->
-    search_from r (next_str i) (pref_str i) = None.
-Proof.
-  intros [next pref] r inp Hsubset Hsearch Hprefix.
-  generalize dependent pref.
-  induction next; intros pref Hprefix.
-  - simpl; erewrite input_search_exec_none; eauto using ip_eq.
-  - simpl in *.
-    erewrite IHnext. erewrite input_search_exec_none.
-    all: eauto using ip_prev'.
-Qed.
-
-Lemma input_search_exec_impossible {strs:StrSearch} {engine:Engine}:
-  forall inp r,
-    supported_regex r ->
-    extract_literal r = Impossible ->
-    exec r inp = None.
-Proof.
-  intros inp r Hsubset Hextract.
-  rewrite <-exec_correct; [|assumption].
-  pose proof (is_tree_productivity r inp Groups.GroupMap.empty forward) as [tree Htree].
-  eauto using extract_literal_impossible.
-Qed.
-
-Lemma search_from_impossible_prefix {strs:StrSearch} {engine:Engine}:
-  forall inp r,
-    supported_regex r ->
-    extract_literal r = Impossible ->
-    search_from r (next_str inp) (pref_str inp) = None.
-Proof.
-  intros [next pref] r Hsubset Hextract.
-  generalize dependent pref.
-  induction next; intros pref; simpl; erewrite input_search_exec_impossible; eauto.
-Qed.
-
-Theorem builtin_exec_equiv {strs:StrSearch} {engine:Engine}:
-  forall r inp,
-    supported_regex r ->
-    BuiltinExec r inp = BuiltinExecPrefixed r inp.
-Proof.
-  intros r inp Hsubset.
-  unfold BuiltinExec, BuiltinExecPrefixed.
-  wt_eq.
-  + eapply search_from_impossible_prefix; eauto.
-  + destruct input_search eqn:Hsearch.
-    - assert (input_prefix inp i). {
-        apply input_search_strict_suffix in Hsearch.
-        now rewrite <-input_prefix_strict_suffix in Hsearch.
-      }
-      eapply search_from_before_jump_eq; eauto using ip_eq.
-    - eapply search_from_none_prefix; eauto using ip_eq.
-Qed.
-
-(* TODO: replace with theorem where the fuel is derived from the complexity of the PikeVM *)
-Axiom pike_vm_fuel: forall r inp, pike_vm_match rer r inp <> OutOfFuel.
-
-(* we show that the PikeVM fits the scheme of an engine *)
-#[refine]
-Instance PikeVMEngine: Engine := {
-  exec r inp := match pike_vm_match rer r inp with
-                | OutOfFuel => None
-                | Finished res => res
-                end;
-  supported_regex := pike_regex;
-}.
-  (* exec_correct *)
-  intros r inp ol Hsubset.
-  destruct pike_vm_match eqn:Hmatch; [pose proof pike_vm_fuel r inp; contradiction|].
-  split.
-  - intros [tree [Htree Hleaf]].
-    subst. eauto using pike_vm_match_correct, pike_vm_correct.
-  - intros ?; subst.
-    pose proof (is_tree_productivity r inp Groups.GroupMap.empty forward) as [tree Htree].
-    exists tree.
-    split; eauto.
-    symmetry. eauto using pike_vm_match_correct, pike_vm_correct.
-Qed.
-
-End PrefixedEngine.
 End Prefix.
