Engine/Meta.v
@@ -1,0 +1,224 @@
+Require Import List.
+Import ListNotations.
+
+From Linden Require Import Regex Chars Semantics Tree.
+From Linden Require Import FunctionalUtils FunctionalSemantics.
+From Linden Require Import Parameters LWParameters.
+From Linden Require Import StrictSuffix Prefix.
+From Linden Require Import PikeSubset SeenSets.
+From Linden Require Import Correctness FunctionalPikeVM.
+From Warblre Require Import Base RegExpRecord.
+
+
+Section Meta.
+	Context {params: LindenParameters}.
+  Context (rer: RegExpRecord).
+
+Section Engines.
+  Context {VMS: VMSeen}.
+
+(* interface of an anchored, executable engine *)
+Class AnchoredEngine := {
+  exec: regex -> input -> option leaf;
+
+  (* asserts the supported subset of regexes *)
+  supported_regex: regex -> Prop;
+
+  (* the execution follows the backtracking tree semantics *)
+  exec_correct: forall r inp ol,
+    supported_regex r ->
+      ((exists tree,
+        is_tree rer [Areg r] inp Groups.GroupMap.empty forward tree /\
+        first_leaf tree inp = ol) <->
+      exec r inp = ol)
+}.
+
+(* we show that the PikeVM fits the scheme of an anchored engine *)
+#[refine]
+Instance PikeVMAnchoredEngine: AnchoredEngine := {
+  exec r inp := match pike_vm_match rer r inp with
+                | OutOfFuel => None
+                | Finished res => res
+                end;
+  supported_regex := pike_regex;
+}.
+  (* exec_correct *)
+  intros r inp ol Hsubset.
+	pose proof (pike_vm_match_terminates rer r inp Hsubset) as [res Hmatch].
+	rewrite Hmatch.
+  split.
+  - intros [tree [Htree Hleaf]].
+    subst. eauto using pike_vm_match_correct, pike_vm_correct.
+  - intros ?; subst.
+    pose proof (is_tree_productivity rer [Areg r] inp Groups.GroupMap.empty forward) as [tree Htree].
+    exists tree.
+    split; eauto.
+    symmetry. eauto using pike_vm_match_correct, pike_vm_correct.
+Qed.
+End Engines.
+
+(* relation that one input is a non-strict prefix of another *)
+Inductive input_prefix : input -> input -> Prop :=
+| ip_eq : forall inp, input_prefix inp inp
+| ip_prev : forall inp1 inp2 inp3,
+    advance_input inp1 forward = Some inp2 ->
+    input_prefix inp2 inp3 ->
+    input_prefix inp1 inp3.
+
+Lemma ip_prev':
+  forall inp1 inp2 inp3,
+    input_prefix inp1 inp2 ->
+    advance_input inp2 forward = Some inp3 ->
+    input_prefix inp1 inp3.
+Proof. induction 1; eauto using ip_prev, ip_eq. Qed.
+
+(* equivalence between input_prefix and strict_suffix *)
+Lemma input_prefix_strict_suffix:
+  forall i1 i2,
+    input_prefix i1 i2 <->
+      i2 = i1 \/ strict_suffix i2 i1 forward.
+Proof.
+  split; intros H.
+  - induction H; [auto|].
+    destruct IHinput_prefix; subst; eauto using ss_advance, ss_next'.
+  - destruct H; [subst; auto using ip_eq|].
+    remember forward as dir.
+    induction H; subst; eauto using ip_eq, ip_prev, ip_prev'.
+Qed.
+
+Existing Instance literal_EqDec.
+(* for each input position we run the engine and return the earliest match *)
+Fixpoint search_from {engine:AnchoredEngine} (r: regex) (next: string) (prev: string): option leaf :=
+  match (exec r (Input next prev)) with
+  | Some leaf => Some leaf
+  | None => match next with
+            | [] => None
+            | c::t => search_from r t (c::prev)
+            end
+  end.
+
+Definition pref_str (i: input) : string :=
+  match i with
+  | Input _ pref => pref
+  end.
+
+(* the string-quadratic algorithm described in RegExpBuiltinExec *)
+Definition BuiltinExec {engine:AnchoredEngine} (r:regex) (inp:input) : option leaf :=
+  search_from r (next_str inp) (pref_str inp).
+
+(* prefixed version *)
+Definition BuiltinExecPrefixed {strs:StrSearch} {engine:AnchoredEngine} (r:regex) (inp:input) : option leaf :=
+  let lit := extract_literal rer r in
+  if lit == Impossible then None else
+    let p := prefix lit in
+    (* we skip the initial input that does not match the prefix *)
+    match (input_search p inp) with
+    | None => None (* if prefix is not present anywhere, then we cannot match *)
+    | Some i => search_from r (next_str i) (pref_str i)
+    end.
+
+Lemma search_from_before_jump_eq {strs:StrSearch} {engine:AnchoredEngine}:
+  forall i r inp inp',
+    supported_regex r ->
+    input_search (prefix (extract_literal rer r)) inp = Some inp' ->
+    input_prefix i inp' ->
+    input_prefix inp i ->
+    search_from r (next_str i) (pref_str i) = search_from r (next_str inp') (pref_str inp').
+Proof.
+  intros i r inp inp' Hsubset Hsearch Hprefix Hlow.
+  induction Hprefix.
+  - reflexivity.
+  - pose proof H as Hadvance.
+    specialize (IHHprefix Hsearch).
+    unfold advance_input in H. destruct inp1 as [next1 pref1] eqn:Hinp1, next1 eqn:Hnext1; [easy|].
+    inversion H. rewrite <-H1 in IHHprefix.
+
+    assert (Hnone: exec r (Input (t :: s) pref1) = None). {
+      assert (Hbetween: input_between inp inp3 inp1). {
+        rewrite input_prefix_strict_suffix in Hprefix, Hlow.
+        split; destruct Hprefix, Hlow; subst; eauto using ss_next', ss_advance.
+      }
+
+      subst.
+      pose proof (is_tree_productivity rer [Areg r] (Input (t :: s) pref1) Groups.GroupMap.empty forward) as [tree Htree].
+      rewrite <-exec_correct; [|assumption].
+      eauto using input_search_no_earlier, extract_literal_prefix_contra.
+    }
+    simpl.
+    rewrite Hnone.
+    eauto using ip_prev'.
+Qed.
+
+Lemma input_search_exec_none {strs:StrSearch} {engine:AnchoredEngine}:
+  forall i r inp,
+    supported_regex r ->
+    input_search (prefix (extract_literal rer r)) inp = None ->
+    input_prefix inp i ->
+    exec r i = None.
+Proof.
+  intros i r inp Hsubset Hsearch Hlow.
+  rewrite input_prefix_strict_suffix in Hlow.
+  rewrite <-exec_correct; [|assumption].
+  pose proof (is_tree_productivity rer [Areg r] i Groups.GroupMap.empty forward) as [tree Htree].
+  eauto using input_search_not_found, extract_literal_prefix_contra.
+Qed.
+
+Lemma search_from_none_prefix {strs:StrSearch} {engine:AnchoredEngine}:
+  forall i r inp,
+    supported_regex r ->
+    input_search (prefix (extract_literal rer r)) inp = None ->
+    input_prefix inp i ->
+    search_from r (next_str i) (pref_str i) = None.
+Proof.
+  intros [next pref] r inp Hsubset Hsearch Hprefix.
+  generalize dependent pref.
+  induction next; intros pref Hprefix.
+  - simpl; erewrite input_search_exec_none; eauto using ip_eq.
+  - simpl in *.
+    erewrite IHnext. erewrite input_search_exec_none.
+    all: eauto using ip_prev'.
+Qed.
+
+Lemma input_search_exec_impossible {strs:StrSearch} {engine:AnchoredEngine}:
+  forall inp r,
+    supported_regex r ->
+    extract_literal rer r = Impossible ->
+    exec r inp = None.
+Proof.
+  intros inp r Hsubset Hextract.
+  rewrite <-exec_correct; [|assumption].
+  pose proof (is_tree_productivity rer [Areg r] inp Groups.GroupMap.empty forward) as [tree Htree].
+  eauto using extract_literal_impossible.
+Qed.
+
+Lemma search_from_impossible_prefix {strs:StrSearch} {engine:AnchoredEngine}:
+  forall inp r,
+    supported_regex r ->
+    extract_literal rer r = Impossible ->
+    search_from r (next_str inp) (pref_str inp) = None.
+Proof.
+  intros [next pref] r Hsubset Hextract.
+  generalize dependent pref.
+  induction next; intros pref; simpl; erewrite input_search_exec_impossible; eauto.
+Qed.
+
+Theorem builtin_exec_equiv {strs:StrSearch} {engine:AnchoredEngine}:
+  forall r inp,
+    supported_regex r ->
+    BuiltinExec r inp = BuiltinExecPrefixed r inp.
+Proof.
+  intros r inp Hsubset.
+  unfold BuiltinExec, BuiltinExecPrefixed.
+  wt_eq.
+  + eapply search_from_impossible_prefix; eauto.
+  + destruct input_search eqn:Hsearch.
+    - assert (input_prefix inp i). {
+        apply input_search_strict_suffix in Hsearch.
+        now rewrite <-input_prefix_strict_suffix in Hsearch.
+      }
+      eapply search_from_before_jump_eq; eauto using ip_eq.
+    - eapply search_from_none_prefix; eauto using ip_eq.
+Qed.
+
+
+End Meta.
